Prove rmw to llsc

src/promising/RMWtoLLSC.v
@@ -33,7 +33,7 @@ Fixpoint rmw_to_llsc_stmt (tmp1 tmp2: Id.t) (stmt: stmtT): list stmtT :=
     [stmt_dowhile
        [stmt_instr (instr_load true ordr tmp1 eloc);
         stmt_instr (instr_store true ordw tmp2 eloc (expr_op2 op_add (expr_reg tmp1) eadd))]
-       (expr_op1 op_not (expr_reg tmp1));
+       (expr_op1 op_not (expr_reg tmp2));
      stmt_instr (instr_assign res (expr_reg tmp1))]
   | stmt_if cond s1 s2 =>
     [stmt_if cond
@@ -54,22 +54,22 @@ Definition rmw_to_llsc_program (p_src p_tgt: program): Prop :=
       (fun stmts_src stmts_tgt => stmts_tgt = rmw_to_llsc_stmts tmp1 tmp2 stmts_src)
       (IdMap.find tid p_src) (IdMap.find tid p_tgt).
 
-Inductive fresh (r: Id.t): forall (stmt: stmtT), Prop :=
+Inductive fresh (regs: IdSet.t): forall (stmt: stmtT), Prop :=
 | fresh_instr
     i
-    (FRESH: ~ IdSet.mem r (regs_of_instr i)):
-  fresh r (stmt_instr i)
+    (FRESH: IdSet.disjoint regs (regs_of_instr i)):
+  fresh regs (stmt_instr i)
 | fresh_if
     cond s1 s2
-    (FRESH_COND: ~ IdSet.mem r (regs_of_expr cond))
-    (FRESH_STMT1: List.Forall (fresh r) s1)
-    (FRESH_STMT2: List.Forall (fresh r) s2):
-  fresh r (stmt_if cond s1 s2)
+    (FRESH_COND: IdSet.disjoint regs (regs_of_expr cond))
+    (FRESH_STMT1: List.Forall (fresh regs) s1)
+    (FRESH_STMT2: List.Forall (fresh regs) s2):
+  fresh regs (stmt_if cond s1 s2)
 | fresh_dowhile
     s cond
-    (FRESH_STMT: List.Forall (fresh r) s)
-    (FRESH_COND: ~ IdSet.mem r (regs_of_expr cond)):
-  fresh r (stmt_dowhile s cond)
+    (FRESH_STMT: List.Forall (fresh regs) s)
+    (FRESH_COND: IdSet.disjoint regs (regs_of_expr cond)):
+  fresh regs (stmt_dowhile s cond)
 .
 
 Definition is_exclusive (i: instrT): bool :=
@@ -99,88 +99,387 @@ Inductive exclusive_free: forall (stmt: stmtT), Prop :=
 Variant sim_val (v_src v_tgt: ValA.t (A:=View.t (A:=unit))): Prop :=
 | sim_val_intro
     (VAL: ValA.val v_src = ValA.val v_tgt)
-    (ANNOT: ValA.annot v_src = ValA.annot v_tgt)
+    (ANNOT: le (ValA.annot v_src) (ValA.annot v_tgt))
 .
+#[export] Hint Constructors sim_val: core.
+
+#[export] Program Instance sim_val_PreOrder: PreOrder sim_val.
+Next Obligation.
+  ii. destruct x. econs; ss. refl.
+Qed.
+Next Obligation.
+  ii. inv H. inv H0.
+  destruct x, y, z. ss.
+  econs; ss; try congr.
+  etrans; eauto.
+Qed.
+
+Lemma sim_val_sem_op2
+      op2 v1_src v2_src v1_tgt v2_tgt
+      (SIM1: sim_val v1_src v1_tgt)
+      (SIM2: sim_val v2_src v2_tgt):
+  sim_val (sem_op2 op2 v1_src v2_src) (sem_op2 op2 v1_tgt v2_tgt).
+Proof.
+  inv SIM1. inv SIM2.
+  unfold sem_op2. econs; s; try congr.
+  eapply join_le; try eapply View.order; ss.
+Qed.
 
 Definition sim_rmap (regs: IdSet.t) (rmap_src rmap_tgt: RMap.t (A:=View.t (A:=unit))): Prop :=
   forall r (NEQ: ~ IdSet.In r regs),
     sim_val (RMap.find r rmap_src) (RMap.find r rmap_tgt).
 
+#[export] Program Instance sim_rmap_PreOrder regs: PreOrder (sim_rmap regs).
+Next Obligation.
+  ii. refl.
+Qed.
+Next Obligation.
+  ii. etrans; eauto.
+Qed.
+
+Lemma sim_rmap_sem_expr
+      regs rmap_src rmap_tgt
+      expr
+      (SIM: sim_rmap regs rmap_src rmap_tgt)
+      (EXPR: IdSet.disjoint regs (regs_of_expr expr)):
+  sim_val (sem_expr rmap_src expr) (sem_expr rmap_tgt expr).
+Proof.
+  revert EXPR.
+  induction expr; i; ss.
+  - refl.
+  - apply SIM. ii.
+    eapply EXPR; eauto.
+    eapply IdSet.singleton_2. ss.
+  - apply IHexpr in EXPR. inv EXPR.
+    unfold sem_op1. econs; s; congr.
+  - exploit IHexpr1; ii.
+    { eauto using IdSet.union_2. }
+    exploit IHexpr2; ii.
+    { eauto using IdSet.union_3. }
+    inv x0. inv x1.
+    unfold sem_op2. econs; s; try congr.
+    eapply join_le; try eapply View.order; ss.
+Qed.
+
+Lemma sim_rmap_add
+      regs rmap_src rmap_tgt
+      r v_src v_tgt
+      (RMAP: sim_rmap regs rmap_src rmap_tgt)
+      (VAL: sim_val v_src v_tgt):
+  sim_rmap regs (RMap.add r v_src rmap_src) (RMap.add r v_tgt rmap_tgt).
+Proof.
+  ii. do 2 rewrite RMap.add_o.
+  condtac; ss; eauto.
+Qed.
+
+Lemma sim_rmap_add_l
+      regs rmap_src rmap_tgt
+      r v
+      (RMAP: sim_rmap regs rmap_src rmap_tgt)
+      (IN: IdSet.In r regs):
+  sim_rmap regs (RMap.add r v rmap_src) rmap_tgt.
+Proof.
+  ii. rewrite RMap.add_o.
+  condtac; ss; eauto. inversion e. congr.
+Qed.
+
+Lemma sim_rmap_add_r
+      regs rmap_src rmap_tgt
+      r v
+      (RMAP: sim_rmap regs rmap_src rmap_tgt)
+      (IN: IdSet.In r regs):
+  sim_rmap regs rmap_src (RMap.add r v rmap_tgt).
+Proof.
+  ii. rewrite RMap.add_o.
+  condtac; ss; eauto. inversion e. congr.
+Qed.
+
+Variant sim_fwditem (fwd_src fwd_tgt: FwdItem.t (A:=unit)): Prop :=
+| sim_fwditem_intro
+    (TS: FwdItem.ts fwd_src = FwdItem.ts fwd_tgt)
+    (VIEW: le (FwdItem.view fwd_src) (FwdItem.view fwd_tgt))
+    (EX: FwdItem.ex fwd_src = FwdItem.ex fwd_tgt)
+.
+#[export] Hint Constructors sim_fwditem: core.
+
+#[export] Program Instance sim_fwditem_PreOrder: PreOrder sim_fwditem.
+Next Obligation.
+  ii. destruct x. econs; ss. refl.
+Qed.
+Next Obligation.
+  ii. inv H. inv H0.
+  destruct x, y, z. ss.
+  econs; ss; try congr.
+  etrans; eauto.
+Qed.
+
+Variant sim_exbank (ex_src ex_tgt: Exbank.t (A:=unit)): Prop :=
+| sim_exbank_intro
+    (LOC: Exbank.loc ex_src = Exbank.loc ex_tgt)
+    (TS: Exbank.ts ex_src = Exbank.ts ex_tgt)
+    (VIEW: le (Exbank.view ex_src) (Exbank.view ex_tgt))
+.
+#[export] Hint Constructors sim_exbank: core.
+
+#[export] Program Instance sim_exbank_PreOrder: PreOrder sim_exbank.
+Next Obligation.
+  ii. destruct x. econs; ss. refl.
+Qed.
+Next Obligation.
+  ii. inv H. inv H0.
+  destruct x, y, z. ss.
+  econs; ss; try congr.
+  etrans; eauto.
+Qed.
+
+Lemma sim_fwditem_read_view
+      fwd_src fwd_tgt
+      (SIM: sim_fwditem fwd_src fwd_tgt):
+  forall ts ord,
+    le (FwdItem.read_view fwd_src ts ord) (FwdItem.read_view fwd_tgt ts ord).
+Proof.
+  inv SIM. i. unfold FwdItem.read_view.
+  rewrite TS, EX. condtac; ss. refl.
+Qed.
+
 Variant sim_local (lc_src lc_tgt: Local.t (A:=unit)): Prop :=
 | sim_local_intro
-    (COH: lc_src.(Local.coh) = lc_tgt.(Local.coh))
-    (VRN: lc_src.(Local.vrn) = lc_tgt.(Local.vrn))
-    (VWN: lc_src.(Local.vwn) = lc_tgt.(Local.vwn))
-    (VRO: lc_src.(Local.vro) = lc_tgt.(Local.vro))
-    (VWO: lc_src.(Local.vwo) = lc_tgt.(Local.vwo))
-    (VCAP: lc_src.(Local.vcap) = lc_tgt.(Local.vcap))
-    (VREL: lc_src.(Local.vrel) = lc_tgt.(Local.vrel))
-    (FWDBANK: lc_src.(Local.fwdbank) = lc_tgt.(Local.fwdbank))
-    (EXBANK: lc_src.(Local.exbank) = None)
+    (COH: le lc_src.(Local.coh) lc_tgt.(Local.coh))
+    (VRN: le lc_src.(Local.vrn) lc_tgt.(Local.vrn))
+    (VWN: le lc_src.(Local.vwn) lc_tgt.(Local.vwn))
+    (VRO: le lc_src.(Local.vro) lc_tgt.(Local.vro))
+    (VWO: le lc_src.(Local.vwo) lc_tgt.(Local.vwo))
+    (VCAP: le lc_src.(Local.vcap) lc_tgt.(Local.vcap))
+    (VREL: le lc_src.(Local.vrel) lc_tgt.(Local.vrel))
+    (FWDBANK: forall loc, sim_fwditem (lc_src.(Local.fwdbank) loc) (lc_tgt.(Local.fwdbank) loc))
     (PROMISES: Local.promises lc_src = Local.promises lc_tgt)
 .
 #[export] Hint Constructors sim_local: core.
 
-(* Lemma sim_local_step *)
-(*       e tid mem_tgt (lc1_tgt lc2_tgt: Local.t (A:=unit)) *)
-(*       mem_src lc1_src *)
-(*       (LOCAL: lc1_src = lc1_tgt) *)
-(*       (MEMORY: mem_src = mem_tgt) *)
-(*       (STEP_TGT: Local.step e tid mem_tgt lc1_tgt lc2_tgt) *)
-(*       (EXFREE: match e with *)
-(*                | Event.read ex _ _ _ *)
-(*                | Event.write ex _ _ _ _ => ex = false *)
-(*                | _ => True *)
-(*                end): *)
-(*   exists lc2_src, *)
-(*     (<<STEP_SRC: Local.step e tid mem_src lc1_src lc2_src>>) /\ *)
-(*     (<<LOCAL2: lc2_src = lc2_tgt>>). *)
-(* Proof. *)
-(*   subst. destruct lc1_tgt. *)
-(*   inv STEP_TGT; subst. *)
-(*   { (* internal *) *)
-(*     esplits; [econs 1|]; eauto. *)
-(*   } *)
-(*   { (* read *) *)
-(*     inv STEP. ss. *)
-(*     esplits; [econs 2|]. *)
-(*     - ss. *)
-(*     - econs; eauto. *)
-(*     - ss. *)
-(*   } *)
-(*   { (* fulfill *) *)
-(*     inv STEP. ss. *)
-(*     esplits; [econs 3|]. *)
-(*     - ss. *)
-(*     - econs; eauto. ss. *)
-(*       inv WRITABLE. ss. econs; eauto. i. ss. *)
-(*     - ss. *)
-(*   } *)
-(*   { (* write failure *) *)
-(*     inv STEP. ss. *)
-(*   } *)
-(*   { (* fadd *) *)
-(*     inv STEP_READ. ss. *)
-(*     inv STEP_FULFILL. ss. *)
-(*     esplits; [econs 5|]. *)
-(*     - ss. *)
-(*     - econs; eauto. *)
-(*     - econs; eauto. *)
-(*     - ss. *)
-(*   } *)
-(*   { (* isb *) *)
-(*     inv STEP. ss. *)
-(*     esplits; [econs 6|]; ss. *)
-(*   } *)
-(*   { (* dmb *) *)
-(*     inv STEP. ss. *)
-(*     esplits; [econs 7|]; ss. *)
-(*   } *)
-(*   { (* control *) *)
-(*     inv LC. ss. *)
-(*     esplits; [econs 8|]; ss. *)
-(*   }         *)
-(* Qed. *)
+#[export] Program Instance sim_local_PreOrder: PreOrder sim_local.
+Next Obligation.
+  ii. destruct x. econs; refl.
+Qed.
+Next Obligation.
+  ii. inv H. inv H0.
+  destruct x, y, z; ss.
+  econs; ss; try refl; etrans; eauto.
+Qed.
+
+Variant sim_event: forall (e_src e_tgt: Event.t (A:=View.t (A:=unit))), Prop :=
+  | sim_event_internal:
+    sim_event Event.internal Event.internal
+  | sim_event_control
+      ctrl_src ctrl_tgt
+      (CTRL: le ctrl_src ctrl_tgt):
+    sim_event (Event.control ctrl_src) (Event.control ctrl_tgt)
+  | sim_event_read
+      ex ord vloc_src vloc_tgt res_src res_tgt
+      (LOC: sim_val vloc_src vloc_tgt)
+      (RES: sim_val res_src res_tgt):
+    sim_event (Event.read ex ord vloc_src res_src)
+              (Event.read ex ord vloc_tgt res_tgt)
+  | sim_event_write
+      ex ord vloc_src vloc_tgt vval_src vval_tgt res_src res_tgt
+      (LOC: sim_val vloc_src vloc_tgt)
+      (VAL: sim_val vval_src vval_tgt)
+      (RES: sim_val res_src res_tgt):
+    sim_event (Event.write ex ord vloc_src vval_src res_src)
+              (Event.write ex ord vloc_tgt vval_tgt res_tgt)
+  | sim_event_fadd
+      ordr ordw vloc_src vloc_tgt vold_src vold_tgt vnew_src vnew_tgt
+      (LOC: sim_val vloc_src vloc_tgt)
+      (OLD: sim_val vold_src vold_tgt)
+      (NEW: sim_val vnew_src vnew_tgt):
+    sim_event (Event.fadd ordr ordw vloc_src vold_src vnew_src)
+              (Event.fadd ordr ordw vloc_tgt vold_tgt vnew_tgt)
+  | sim_event_barrier
+      b:
+    sim_event (Event.barrier b) (Event.barrier b)
+.
+#[export] Hint Constructors sim_event: core.
+
+#[export] Program Instance sim_event_PreOrder: PreOrder sim_event.
+Next Obligation.
+  ii. destruct x; econs; refl.
+Qed.
+Next Obligation.
+  ii. inv H; inv H0; econs; etrans; eauto.
+Qed.
+
+Lemma le_latest
+      loc ts view_src view_tgt mem
+      (LE: view_src <= view_tgt)
+      (LATEST: Memory.latest loc ts view_tgt mem):
+  Memory.latest loc ts view_src mem.
+Proof.
+  unfold Memory.latest, Memory.no_msgs in *. i.
+  eapply LATEST; eauto. etrans; eauto.
+Qed.
+
+Ltac sim_viewtac :=
+  repeat
+    (try match goal with
+         | [|- orderC _ _] => (try apply View.order); (try apply Time.order)
+         | [|- le ?v ?v] => refl
+         | [|- View._le ?v ?v] => refl
+         | [|- le (join _ _) (join _ _)] => eapply join_le
+         | [|- le (View._join _ _) (View._join _ _)] => eapply join_le
+         | [|- View._le (join _ _) (join _ _)] => eapply join_le
+         | [|- View._le (View._join _ _) (View._join _ _)] => eapply join_le
+         | [|- (join _ _) <= (join _ _)] => eapply join_le
+         | [|- le (ifc ?c _) (ifc ?c _)] =>
+             let cond := fresh "COND" in destruct c eqn:cond; ss
+         | [|- View._le (ifc ?c _) (ifc ?c _)] =>
+             let cond := fresh "COND" in destruct c eqn:cond; ss
+         | [|- le (fun_add _ _ _) (fun_add _ _ _)] => ii; unfold fun_add
+         | [|- ?rel (if ?c then _ else _) (if ?c then _ else _)] =>
+             let cond := fresh "COND" in destruct c eqn:cond; ss
+         | [|- le (FwdItem.read_view _ _ _) (FwdItem.read_view _ _ _)] => eapply sim_fwditem_read_view
+         | [|- View._le (FwdItem.read_view _ _ _) (FwdItem.read_view _ _ _)] => eapply sim_fwditem_read_view
+         | [|- View.ts ?a <= View.ts ?b] =>
+             cut (le a b);
+             try (let h := fresh "X" in intro h; apply h)
+         | [H: (le ?a ?b) |- le (?a ?loc) (?b ?loc)] => apply H
+         | [|- sim_fwditem (fun_add _ _ _ _) (fun_add _ _ _ _)] => unfold fun_add
+         | [|- sim_fwditem (FwdItem.mk _ _ _) (FwdItem.mk _ _ _)] => econs
+         end;
+     ss; eauto; i).
+
+Lemma sim_local_read
+      ex ord vloc_tgt res_tgt ts lc1_tgt mem_tgt lc2_tgt
+      vloc_src mem_src lc1_src
+      (LOCAL: sim_local lc1_src lc1_tgt)
+      (MEMORY: mem_src = mem_tgt)
+      (VLOC: sim_val vloc_src vloc_tgt)
+      (STEP_TGT: Local.read ex ord vloc_tgt res_tgt ts lc1_tgt mem_tgt lc2_tgt):
+  exists res_src lc2_src,
+    (<<STEP_SRC: Local.read ex ord vloc_src res_src ts lc1_src mem_src lc2_src>>) /\
+    (<<RES: sim_val res_src res_tgt>>) /\
+    (<<LOCAL2: sim_local lc2_src lc2_tgt>>) /\
+    (<<EX_TRUE: ex = true -> option_rel sim_exbank lc2_src.(Local.exbank) lc2_tgt.(Local.exbank)>>) /\
+    (<<EX_FALSE: ex = false -> lc1_src.(Local.exbank) = lc2_src.(Local.exbank)>>).
+Proof.
+  destruct lc1_src, lc1_tgt. inv LOCAL. ss.
+  destruct vloc_src, vloc_tgt. inv VLOC. ss. subst.
+  inv STEP_TGT. ss.
+  esplits.
+  - econs; eauto; ss.
+    + eapply le_latest; try exact COH0. sim_viewtac.
+    + eapply le_latest; try exact LATEST. sim_viewtac.
+  - ss. econs; ss. sim_viewtac.
+  - s. econs; ss; sim_viewtac.
+  - s. i. subst. econs; ss. sim_viewtac.
+  - s. i. subst. ss.
+Qed.
+
+Lemma sim_local_fulfill
+      ex ord vloc_tgt vval_tgt res ts tid view_pre_tgt lc1_tgt mem_tgt lc2_tgt
+      vloc_src vval_src mem_src lc1_src
+      (LOCAL: sim_local lc1_src lc1_tgt)
+      (MEMORY: mem_src = mem_tgt)
+      (VLOC: sim_val vloc_src vloc_tgt)
+      (VVAL: sim_val vval_src vval_tgt)
+      (EXBANK: ex = true -> option_rel sim_exbank (Local.exbank lc1_src) (Local.exbank lc1_tgt))
+      (STEP_TGT: Local.fulfill ex ord vloc_tgt vval_tgt res ts tid view_pre_tgt lc1_tgt mem_tgt lc2_tgt):
+  exists view_pre_src lc2_src,
+    (<<STEP_SRC: Local.fulfill ex ord vloc_src vval_src res ts tid view_pre_src lc1_src mem_src lc2_src>>) /\
+    (<<VIEW_PRE_SRC: le view_pre_src view_pre_tgt>>) /\
+    (<<LOCAL2: sim_local lc2_src lc2_tgt>>) /\
+    (<<EXBANK: ex = false -> lc1_src.(Local.exbank) = lc2_src.(Local.exbank)>>).
+Proof.
+  destruct lc1_src, lc1_tgt. inv LOCAL. ss.
+  destruct vloc_src, vloc_tgt. inv VLOC. ss. subst.
+  destruct vval_src, vval_tgt. inv VVAL. ss. subst.
+  inv STEP_TGT. ss.
+  inv WRITABLE. ss.
+  esplits.
+  - econs; eauto; ss.
+    + econs; eauto; ss.
+      * eapply Nat.le_lt_trans; try exact COH0. sim_viewtac.
+      * eapply Nat.le_lt_trans; try exact EXT. sim_viewtac.
+        destruct ex; ss.
+        destruct exbank, exbank0; ss; try refl.
+        apply EXBANK. ss.
+      * destruct ex; ss. i.
+        exploit EX; eauto. i. des. subst.
+        exploit EXBANK; eauto. i. destruct exbank; ss.
+        esplits; eauto.
+        inv x0. rewrite LOC, TS. ss.
+    + ss.
+  - s. sim_viewtac.
+    destruct ex; ss.
+    destruct exbank, exbank0; ss; try refl.
+    apply EXBANK. ss.
+  - s. econs; ss; sim_viewtac.
+  - s. i. subst. ss.
+Qed.
+
+Lemma sim_local_isb
+      lc1_tgt lc2_tgt
+      lc1_src
+      (LOCAL: sim_local lc1_src lc1_tgt)
+      (STEP_TGT: Local.isb lc1_tgt lc2_tgt):
+  exists lc2_src,
+    (<<STEP_SRC: Local.isb lc1_src lc2_src>>) /\
+    (<<LOCAL2: sim_local lc2_src lc2_tgt>>) /\
+    (<<EXBANK: lc1_src.(Local.exbank) = lc2_src.(Local.exbank)>>).
+Proof.
+  destruct lc1_src, lc1_tgt. inv LOCAL. ss.
+  inv STEP_TGT. ss.
+  esplits.
+  - econs; ss.
+  - econs; ss; sim_viewtac.
+  - ss.
+Qed.
+
+Lemma sim_local_dmb
+      rr rw wr ww lc1_tgt lc2_tgt
+      lc1_src
+      (LOCAL: sim_local lc1_src lc1_tgt)
+      (STEP_TGT: Local.dmb rr rw wr ww lc1_tgt lc2_tgt):
+  exists lc2_src,
+    (<<STEP_SRC: Local.dmb rr rw wr ww lc1_src lc2_src>>) /\
+    (<<LOCAL2: sim_local lc2_src lc2_tgt>>) /\
+    (<<EXBANK: lc1_src.(Local.exbank) = lc2_src.(Local.exbank)>>).
+Proof.
+  destruct lc1_src, lc1_tgt. inv LOCAL. ss.
+  inv STEP_TGT. ss.
+  esplits.
+  - econs; ss.
+  - econs; ss; sim_viewtac.
+  - ss.
+Qed.
+
+Lemma sim_local_control
+      (ctrl_tgt: View.t (A:=unit)) lc1_tgt lc2_tgt
+      ctrl_src lc1_src
+      (LOCAL: sim_local lc1_src lc1_tgt)
+      (CTRL: le ctrl_src ctrl_tgt)
+      (STEP_TGT: Local.control ctrl_tgt lc1_tgt lc2_tgt):
+  exists lc2_src,
+    (<<STEP_SRC: Local.control ctrl_src lc1_src lc2_src>>) /\
+    (<<LOCAL2: sim_local lc2_src lc2_tgt>>) /\
+    (<<EXBANK: lc1_src.(Local.exbank) = lc2_src.(Local.exbank)>>).
+Proof.
+  destruct lc1_src, lc1_tgt. inv LOCAL. ss.
+  inv STEP_TGT. ss.
+  esplits.
+  - econs; ss.
+  - econs; ss; sim_viewtac.
+  - ss.
+Qed.
+
+Lemma read_sim_local
+      ex ord vloc res ts lc1 mem (lc2: Local.t (A:=unit))
+      (READ: Local.read ex ord vloc res ts lc1 mem lc2):
+  sim_local lc1 lc2.
+Proof.
+  inv READ. econs; ss;
+    try apply join_l; try refl.
+  ii. unfold fun_add. condtac; try refl.
+  inversion e. subst. apply join_l.
+Qed.
 
 Lemma unfold_rmw_to_llsc_stmts
       tmp1 tmp2 s stmts:
@@ -190,6 +489,25 @@ Proof.
    ss.
 Qed.
 
+(* move *)
+
+Lemma add_eq
+      A `{_: orderC A} r1 r2 v (rmap: RMap.t (A:=A))
+      (REG: r1 = r2):
+  RMap.find r1 (RMap.add r2 v rmap) = v.
+Proof.
+  rewrite RMap.add_o. condtac; ss.
+Qed.
+
+Lemma fold_right_app
+      A (l1 l2: list (list A)):
+  fold_right (@List.app _) [] l1 ++ fold_right (@List.app _) [] l2 =
+  fold_right (@List.app _) [] (l1 ++ l2).
+Proof.
+  induction l1; ss.
+  rewrite <- app_assoc.
+  rewrite IHl1. ss.
+Qed.
 
 Section RMWtoLLSC.
   Hypothesis ARCH: arch = armv8.
@@ -199,12 +517,12 @@ Section RMWtoLLSC.
         stmts_src rmap_src lc_src mem_src
         stmts_tgt rmap_tgt lc_tgt mem_tgt
         (TMP: tmp1 <> tmp2)
-        (FRESH1: List.Forall (fresh tmp1) stmts_src)
-        (FRESH2: List.Forall (fresh tmp2) stmts_src)
+        (FRESH: List.Forall (fresh (IdSet.add tmp2 (IdSet.singleton tmp1))) stmts_src)
         (EXFREE: List.Forall exclusive_free stmts_src)
         (STMTS: stmts_tgt = rmw_to_llsc_stmts tmp1 tmp2 stmts_src)
         (RMAP: sim_rmap (IdSet.add tmp2 (IdSet.singleton tmp1)) rmap_src rmap_tgt)
-        (LOCAL: lc_src = lc_tgt)
+        (LOCAL: sim_local lc_src lc_tgt)
+        (EXBANK: lc_src.(Local.exbank) = None)
         (MEMORY: mem_src = mem_tgt):
     @sim_eu tid
             (ExecUnit.mk (State.mk stmts_src rmap_src) lc_src mem_src)
@@ -215,10 +533,11 @@ Section RMWtoLLSC.
     pfold. red. ss. subst. splits.
     { (* terminal *)
       i. red in TERMINAL_TGT. ss. des.
-      esplits; try refl. red. ss. split; try congr.
-      red in TERMINAL_TGT. red. ss.
-      destruct stmts_src; ss.
-      destruct s; ss. destruct i; ss.
+      esplits; try refl. red. ss. split.
+      - red in TERMINAL_TGT. red. ss.
+        destruct stmts_src; ss.
+        destruct s; ss. destruct i; ss.
+      - inv LOCAL. congr.
     }
 
     i. inv STEP_TGT. inv STEP. ss.
@@ -226,124 +545,175 @@ Section RMWtoLLSC.
     destruct eu2_tgt as [[stmts2_tgt rmap2_tgt] lc2_tgt mem2_tgt]. ss. subst.
     destruct s; cycle 1.
     { (* if *)
-      inv STATE.
+      inv STATE. inv LOCAL0; inv EVENT.
+      inv FRESH. inv H1.
+      inv EXFREE. inv H1.
+      exploit sim_rmap_sem_expr; try exact FRESH_COND; eauto. i. inv x0.
+      exploit sim_local_control; try exact LOCAL; eauto. i. des.
       eexists (ExecUnit.mk _ _ _). splits.
-      { econs 2; try refl. econs.
-        econs; try eapply LOCAL; ss.
-        econs; eauto.
-        admit. (* sem_expr *)
+      { econs 2; try refl. econs. econs; ss.
+        - econs; ss.
+        - econs 8; eauto.
       }
-      condtac; ss.
+      rewrite VAL. condtac; ss.
       - right. eapply CIH; eauto.
-        + admit.
-        + admit.
-        + admit.
-        + admit.
+        + rewrite List.Forall_app. split; ss.
+        + rewrite List.Forall_app. split; ss.
+        + rewrite fold_right_app.
+          rewrite <- map_app. ss.
+        + congr.
       - right. eapply CIH; eauto.
-        + admit.
-        + admit.
-        + admit.
-        + admit.
+        + rewrite List.Forall_app. split; ss.
+        + rewrite List.Forall_app. split; ss.
+        + rewrite fold_right_app.
+          rewrite <- map_app. ss.
+        + congr.
     }
 
     { (* while *)
-      inv STATE.
+      inv STATE. inv LOCAL0; inv EVENT.
       eexists (ExecUnit.mk _ _ _). splits.
-      { econs 2; try refl. econs.
-        econs; try eapply LOCAL; ss.
-        econs; eauto.
+      { econs 2; try refl. econs. econs; ss.
+        - econs. ss.
+        - econs 1; eauto.
       }
       right. eapply CIH; eauto.
-      - admit.
-      - admit.
-      - admit.
-      - admit.
+      - inv FRESH. inv H1.
+        rewrite List.Forall_app. split; ss.
+        repeat (econs; ss).
+      - inv EXFREE. inv H1.
+        rewrite List.Forall_app. split; ss.
+        repeat (econs; ss).
+      - unfold rmw_to_llsc_stmts.
+        rewrite map_app.
+        rewrite <- fold_right_app. ss.
     }
 
-    inv FRESH1. inv FRESH2. inv EXFREE.
+    inv FRESH. inv EXFREE.
     rewrite unfold_rmw_to_llsc_stmts in STATE.
     destruct i; ss.
     { (* skip *)
-      inv STATE.
+      inv STATE. inv LOCAL0; inv EVENT.
       eexists (ExecUnit.mk _ _ _). splits.
-      { econs 2; try refl. econs.
-        econs; try eapply LOCAL; ss.
-        econs.
+      { econs 2; try refl. econs. econs; ss.
+        - econs.
+        - econs 1; eauto.
       }
       right. eapply CIH; eauto.
     }
 
     { (* assign *)
-      inv STATE.
+      inv STATE. inv LOCAL0; inv EVENT.
       eexists (ExecUnit.mk _ _ _). splits.
-      { econs 2; try refl. econs.
-        econs; try eapply LOCAL; ss.
-        econs; eauto.
+      { econs 2; try refl. econs. econs; ss.
+        - econs. ss.
+        - econs 1; ss.
       }
       right. eapply CIH; eauto.
-      admit.
+      apply sim_rmap_add; auto.
+      eapply sim_rmap_sem_expr; eauto.
+      inv H1. ii. ss.
+      eapply FRESH; eauto.
+      apply IdSet.add_2. ss.
     }
 
     { (* load *)
-      inv STATE.
+      inv STATE. inv LOCAL0; inv EVENT.
+      exploit sim_local_read; try exact LOCAL; eauto.
+      { eapply sim_rmap_sem_expr; eauto.
+        inv H1. ss. ii. eapply FRESH; eauto.
+        apply IdSet.add_2. ss.
+      }
+      i. des.
       eexists (ExecUnit.mk _ _ _). splits.
-      { econs 2; try refl. econs.
-        econs; try eapply LOCAL; ss.
-        econs; eauto.
-        admit.
+      { econs 2; try refl. econs. econs; ss.
+        - econs; eauto.
+        - econs 2; eauto.
       }
       right. eapply CIH; eauto.
-      admit.
+      - apply sim_rmap_add; ss.
+      - inv H3. ss. destruct ex0; ss.
+        rewrite <- EX_FALSE; ss.
     }
 
     { (* store *)
-      inv STATE.
+      inv STATE. inv LOCAL0; inv EVENT; cycle 1.
+      { inv STEP. inv H3. ss. }
+      exploit sim_local_fulfill; try exact LOCAL; eauto.
+      { eapply sim_rmap_sem_expr; eauto.
+        inv H1. ss. ii. eapply FRESH; eauto.
+        apply IdSet.add_2, IdSet.union_2. ss.
+      }
+      { eapply sim_rmap_sem_expr; eauto.
+        inv H1. ss. ii. eapply FRESH; eauto.
+        apply IdSet.add_2, IdSet.union_3. ss.
+      }
+      { i. subst. inv H3. ss. }
+      i. des.
       eexists (ExecUnit.mk _ _ _). splits.
-      { econs 2; try refl. econs.
-        econs; try eapply LOCAL; ss.
-        econs; eauto.
-        - admit.
-        - admit.
+      { econs 2; try refl. econs. econs; ss.
+        - econs; ss.
+        - econs 3; eauto.
       }
       right. eapply CIH; eauto.
-      admit.
+      - apply sim_rmap_add; ss. refl.
+      - inv H3. ss. destruct ex0; ss.
+        rewrite <- EXBANK0; ss.
     }
 
     { (* fadd *)
-      (* dowhile *)
-      inv STATE. inv LOCAL; ss. clear EVENT.
+      inv STATE. inv LOCAL0; inv EVENT.
       esplits; [refl|]. left.
+      rename rmap2_tgt into rmap_tgt.
+      revert rmap_tgt lc_tgt RMAP LOCAL.
+      pcofix CIH_LOOP. i.
       pfold. red. s. splits.
       { i. repeat (red in TERMINAL_TGT; des; ss). }
 
       (* exclusive load *)
-      i. rename rmap2_tgt into rmap_tgt.
-      destruct eu2_tgt as [[]].
+      i. destruct eu2_tgt as [[]].
       inv STEP_TGT. inv STEP. ss. subst.
-      inv STATE. inv LOCAL; inv EVENT.
+      inv STATE. inv LOCAL0; inv EVENT.
       esplits; [refl|]. left.
-
-      revert ts res0 local STEP.
-      pcofix CIH_LOOP. i.
       pfold. red. s. splits.
       { i. repeat (red in TERMINAL_TGT; des; ss). }
 
       (* exclusive store *)
       i. destruct eu2_tgt as [[]].
       inv STEP_TGT. inv STEP0. ss. subst.
-      inv STATE. inv LOCAL; inv EVENT.
+      inv STATE. inv LOCAL0; inv EVENT.
 
       { (* exclusive store - succeed *)
         clear CIH_LOOP.
+        exploit sim_local_read; try exact STEP; eauto.
+        { eapply sim_rmap_sem_expr; eauto.
+          inv H1. ss. ii. eapply FRESH; eauto.
+          apply IdSet.add_2, IdSet.union_2. ss.
+        }
+        i. des.
+        exploit sim_local_fulfill; try exact STEP0; eauto.
+        { eapply sim_rmap_sem_expr.
+          - eapply sim_rmap_add_r; eauto.
+            apply IdSet.add_2, IdSet.singleton_2. ss.
+          - inv H1. ss. ii.
+            eapply FRESH; eauto.
+            apply IdSet.add_2, IdSet.union_2. ss.
+        }
+        { apply sim_val_sem_op2.
+          - rewrite RMap.add_o. condtac; try congr. eauto.
+          - eapply sim_rmap_sem_expr.
+            + eapply sim_rmap_add_r; eauto.
+              apply IdSet.add_2, IdSet.singleton_2. ss.
+            + inv H1. ss. ii.
+              eapply FRESH; eauto.
+              apply IdSet.add_2, IdSet.union_3. ss.
+        }
+        i. des.
         eexists (ExecUnit.mk _ _ _). splits.
-        { econs 2; try refl. econs. econs; cycle 1.
-          - s. econs 5; try exact STEP; eauto.
-            replace (sem_expr rmap_tgt eloc) with (sem_expr (RMap.add tmp1 res0 rmap_tgt) eloc); eauto.
-            admit.
-          - ss.
+        { econs 2; try refl. econs. econs; s.
           - econs; eauto.
-            + admit.
-            + admit.
+          - econs 5; eauto.
+          - ss.
         }
         left. pfold. red. s. splits.
         { i. repeat (red in TERMINAL_TGT; des; ss). }
@@ -351,11 +721,22 @@ Section RMWtoLLSC.
         (* if *)
         i. destruct eu2_tgt as [[]].
         inv STEP_TGT. inv STEP1. ss. subst.
-        inv STATE. inv LOCAL; inv EVENT.
+        inv STATE. inv LOCAL1; inv EVENT.
         condtac; ss.
-        { admit. }
+        { exfalso. apply c.
+          rewrite RMap.add_o. condtac; try congr.
+          inv STEP_SRC0. ss.
+        }
         clear e X.
-        replace local1 with local0 in * by admit.
+        replace local1 with local0 in *; cycle 1.
+        { destruct local0, local1.
+          inv LC; ss. inv LC2. f_equal.
+          rewrite RMap.add_o. condtac; try congr.
+          inv STEP_SRC0. ss. rewrite ARCH. ss.
+          rewrite bot_join; ss.
+          destruct view_pre_src. destruct annot. ss.
+          apply View.order.
+        }
         clear local1 LC.
         esplits; [refl|].
         left. pfold. red. s. splits.
@@ -364,11 +745,19 @@ Section RMWtoLLSC.
         (* assign *)
         i. destruct eu2_tgt as [[]].
         inv STEP_TGT. inv STEP1. ss. subst.
-        inv STATE. inv LOCAL; inv EVENT.
+        inv STATE. inv LOCAL1; inv EVENT.
         esplits; [refl|].
         right. eapply CIH; eauto.
         - rewrite List.app_nil_r. ss.
-        - admit.
+        - apply sim_rmap_add.
+          + apply sim_rmap_add_r; cycle 1.
+            { apply IdSet.add_1. ss. }
+            apply sim_rmap_add_r; ss.
+            apply IdSet.add_2. apply IdSet.singleton_2. ss.
+          + unfold sem_expr.
+            rewrite RMap.add_o. condtac; ss.
+            rewrite RMap.add_o. condtac; try congr.
+        - inv STEP_SRC0. ss.
       }
 
       { (* exclusive store - fail *)
@@ -380,11 +769,10 @@ Section RMWtoLLSC.
         (* if *)
         i. destruct eu2_tgt as [[]].
         inv STEP_TGT. inv STEP0. ss. subst.
-        inv STATE. inv LOCAL; inv EVENT. inv LC. ss.
-        rewrite RMap.add_o. destruct (tmp == tmp); try congr. ss.
+        inv STATE. inv LOCAL0; inv EVENT. inv LC. ss.
+        repeat rewrite add_eq; ss.
         replace (join (Local.vcap local) bot) with (Local.vcap local); cycle 1.
         { rewrite bot_join; ss. apply View.order. }
-        clear e.
         esplits; try refl. left.
         pfold. red. ss. splits.
         { i. repeat (red in TERMINAL_TGT; des; ss). }
@@ -392,47 +780,57 @@ Section RMWtoLLSC.
         (* dowhile *)
         i. destruct eu2_tgt as [[]].
         inv STEP_TGT. inv STEP0. ss. subst.
-        inv STATE. inv LOCAL; inv EVENT.
-        esplits; [refl|]. left.
-        pfold. red. s. splits.
-        { i. repeat (red in TERMINAL_TGT; des; ss). }
-
-        (* load *)
-        i. destruct eu2_tgt as [[]].
-        inv STEP_TGT. inv STEP0. ss. subst.
-        inv STATE. inv LOCAL; inv EVENT.
-        admit.
+        inv STATE. inv LOCAL0; inv EVENT. ss.
+        esplits; [refl|]. right.
+        repeat rewrite List.app_nil_r.
+        eapply CIH_LOOP.
+        - apply sim_rmap_add_r; cycle 1.
+          { apply IdSet.add_1. ss. }
+          apply sim_rmap_add_r; ss.
+          apply IdSet.add_2. apply IdSet.singleton_2. ss.
+        - exploit read_sim_local; try exact STEP. i.
+          etrans; eauto. etrans; eauto.
+          destruct local. ss.
+          econs; s; refl.
       }
     }
 
     { (* barrier *)
-      inv STATE.
-      eexists (ExecUnit.mk _ _ _). splits.
-      { econs 2; try refl. econs.
-        econs; try eapply STEP_SRC; ss.
-        econs.
-      }
-      right. eapply CIH; eauto.
+      inv STATE. inv LOCAL0; inv EVENT.
+      - exploit sim_local_isb; eauto. i. des.
+        eexists (ExecUnit.mk _ _ _). splits.
+        { econs 2; try refl. econs. econs; ss.
+          - econs; ss.
+          - econs 6; eauto.
+        }
+        right. eapply CIH; eauto. congr.
+      - exploit sim_local_dmb; eauto. i. des.
+        eexists (ExecUnit.mk _ _ _). splits.
+        { econs 2; try refl. econs. econs; ss.
+          - econs; ss.
+          - econs 7; eauto.
+        }
+        right. eapply CIH; eauto. congr.
     }
-  Admitted.
+  Qed.
 End RMWtoLLSC.
 
 
-Variant sim_sl (tmp: Id.t):
+Variant sim_sl (tmp1 tmp2: Id.t):
   forall (sl_src sl_tgt: State.t (A:=View.t (A:=unit)) * Local.t (A:=unit)), Prop :=
 | sim_sl_intro
     stmts_src rmap_src lc_src
     stmts_tgt rmap_tgt lc_tgt
-    (STMTS: stmts_tgt = rmw_to_llsc_stmts tmp stmts_src)
-    (RMAP: sim_rmap tmp rmap_src rmap_tgt)
-    (LOCAL: lc_src = lc_tgt) (* TODO: fix *):
-  sim_sl tmp (State.mk stmts_src rmap_src, lc_src) (State.mk stmts_tgt rmap_tgt, lc_tgt)
+    (STMTS: stmts_tgt = rmw_to_llsc_stmts tmp1 tmp2 stmts_src)
+    (RMAP: sim_rmap (IdSet.add tmp2 (IdSet.singleton tmp1)) rmap_src rmap_tgt)
+    (LOCAL: sim_local lc_src lc_tgt):
+  sim_sl tmp1 tmp2 (State.mk stmts_src rmap_src, lc_src) (State.mk stmts_tgt rmap_tgt, lc_tgt)
 .
 
 Variant sim_machine (m_src m_tgt: Machine.t): Prop :=
 | sim_machine_intro
-    (TPOOL: forall tid, exists tmp,
-        option_rel (sim_sl tmp)
+    (TPOOL: forall tid, exists tmp1 tmp2,
+        option_rel (sim_sl tmp1 tmp2)
                    (IdMap.find tid (Machine.tpool m_src))
                    (IdMap.find tid (Machine.tpool m_tgt)))
     (MEMORY: Machine.mem m_src = Machine.mem m_tgt)
